HOL/DataStrs/RBTree.thy
@@ -1,6 +1,6 @@
 (* Verification of functional red-black trees. *)
 
-theory RBT
+theory RBTree
 imports Lists_Ex
 begin
 
@@ -151,7 +151,7 @@ setup {* fold del_prfstep_thm (@{thms rbt_set.simps} @ @{thms rbt_sorted.simps})
 
 section {* Balance function *}
 
-definition balanceR :: "('a, 'b) rbt \<Rightarrow> 'a \<Rightarrow> 'b \<Rightarrow> ('a, 'b) rbt \<Rightarrow> ('a, 'b) rbt" where [rewrite]:
+definition balanceR :: "('a, 'b) rbt \<Rightarrow> 'a \<Rightarrow> 'b \<Rightarrow> ('a, 'b) rbt \<Rightarrow> ('a, 'b) rbt" where [rewrite,unfold]:
   "balanceR l k v r =
    (if cl r = R then
       let lr = lsub r; rr = rsub r in
@@ -160,7 +160,7 @@ definition balanceR :: "('a, 'b) rbt \<Rightarrow> 'a \<Rightarrow> 'b \<Rightar
       else Node l B k v r
     else Node l B k v r)"
   
-definition balance :: "('a, 'b) rbt \<Rightarrow> 'a \<Rightarrow> 'b \<Rightarrow> ('a, 'b) rbt \<Rightarrow> ('a, 'b) rbt" where [rewrite]:
+definition balance :: "('a, 'b) rbt \<Rightarrow> 'a \<Rightarrow> 'b \<Rightarrow> ('a, 'b) rbt \<Rightarrow> ('a, 'b) rbt" where [rewrite,unfold]:
   "balance l k v r =
    (if cl l = R then
       let ll = lsub l; rl = rsub l in
@@ -279,7 +279,7 @@ theorem rbt_search_correct [rewrite]:
     
 section {* balL and balR *}
 
-definition balL :: "('a, 'b) rbt \<Rightarrow> 'a \<Rightarrow> 'b \<Rightarrow> ('a, 'b) rbt \<Rightarrow> ('a, 'b) rbt" where [rewrite]:
+definition balL :: "('a, 'b) rbt \<Rightarrow> 'a \<Rightarrow> 'b \<Rightarrow> ('a, 'b) rbt \<Rightarrow> ('a, 'b) rbt" where [rewrite,unfold]:
   "balL l k v r = (let lr = lsub r in
    if cl l = R then Node (Node (lsub l) B (key l) (val l) (rsub l)) R k v r
    else if r = Leaf then Node l R k v r
@@ -291,7 +291,7 @@ definition balL :: "('a, 'b) rbt \<Rightarrow> 'a \<Rightarrow> 'b \<Rightarrow>
 setup {* register_wellform_data ("balL l k v r", ["black_depth l + 1 = black_depth r"]) *}
 setup {* add_prfstep_check_req ("balL l k v r", "black_depth l + 1 = black_depth r") *}
   
-definition balR :: "('a, 'b) rbt \<Rightarrow> 'a \<Rightarrow> 'b \<Rightarrow> ('a, 'b) rbt \<Rightarrow> ('a, 'b) rbt" where [rewrite]:
+definition balR :: "('a, 'b) rbt \<Rightarrow> 'a \<Rightarrow> 'b \<Rightarrow> ('a, 'b) rbt \<Rightarrow> ('a, 'b) rbt" where [rewrite,unfold]:
   "balR l k v r = (let rl = rsub l in
    if cl r = R then Node l R k v (Node (lsub r) B (key r) (val r) (rsub r))
    else if l = Leaf then Node l R k v r
@@ -364,7 +364,8 @@ fun combine :: "('a, 'b) rbt \<Rightarrow> ('a, 'b) rbt \<Rightarrow> ('a, 'b) r
            balL l1 k1 v1 (Node tm B k2 v2 r2)
      else
        Node (combine (Node l1 c1 k1 v1 r1) l2) R k2 v2 r2)"
-setup {* fold add_rewrite_rule @{thms combine.simps} *}
+setup {* fold add_rewrite_rule @{thms combine.simps(1,2)} *}
+setup {* add_unfolding_rule @{thm combine.simps(3)} *}
 setup {* add_fun_induct_rule (@{term combine}, @{thm combine.induct}) *}
 
 lemma combine_bd:
@@ -372,8 +373,9 @@ lemma combine_bd:
    bd_inv (combine lt rt) \<and> black_depth (combine lt rt) = black_depth lt"
 @proof @fun_induct "combine lt rt" @with
   @subgoal "(lt = Node l1 c1 k1 v1 r1, rt = Node l2 c2 k2 v2 r2)"
-  @case "c1 = B" @with @case "c2 = B" @with @case "cl (combine r1 l2) = B" @with
-    @have "cl (Node (combine r1 l2) B k2 v2 r2) = B" @end @end @end
+    @unfold "combine (Node l1 c1 k1 v1 r1) (Node l2 c2 k2 v2 r2)"
+    @case "c1 = B" @with @case "c2 = B" @with @case "cl (combine r1 l2) = B" @with
+      @have "cl (Node (combine r1 l2) B k2 v2 r2) = B" @end @end @end
   @endgoal @end
 @qed
 setup {* add_forward_prfstep_cond @{thm combine_bd} [with_term "combine ?lt ?rt"] *}
@@ -383,8 +385,9 @@ lemma combine_cl:
    (cl lt = B \<longrightarrow> cl rt = B \<longrightarrow> cl_inv (combine lt rt)) \<and> cl_inv' (combine lt rt)"
 @proof @fun_induct "combine lt rt" @with
   @subgoal "(lt = Node l1 c1 k1 v1 r1, rt = Node l2 c2 k2 v2 r2)"
-  @case "c1 = B" @with @case "c2 = B" @with @case "cl (combine r1 l2) = B" @with
-    @have "cl (Node (combine r1 l2) B k2 v2 r2) = B" @end @end @end
+    @unfold "combine (Node l1 c1 k1 v1 r1) (Node l2 c2 k2 v2 r2)"
+    @case "c1 = B" @with @case "c2 = B" @with @case "cl (combine r1 l2) = B" @with
+      @have "cl (Node (combine r1 l2) B k2 v2 r2) = B" @end @end @end
   @endgoal @end
 @qed
 setup {* add_forward_prfstep_cond @{thm combine_cl} [with_term "combine ?lt ?rt"] *}
@@ -393,6 +396,7 @@ lemma combine_in_traverse_pairs [rewrite]:
   "rbt_in_traverse_pairs (combine lt rt) = rbt_in_traverse_pairs lt @ rbt_in_traverse_pairs rt"
 @proof @fun_induct "combine lt rt" @with
   @subgoal "(lt = Node l1 c1 k1 v1 r1, rt = Node l2 c2 k2 v2 r2)"
+    @unfold "combine (Node l1 c1 k1 v1 r1) (Node l2 c2 k2 v2 r2)"
     @case "c1 = R" @with @case "c2 = R" @with @case "cl (combine r1 l2) = R" @with
       @have "rbt_in_traverse_pairs (combine (Node l1 c1 k1 v1 r1) (Node l2 c2 k2 v2 r2)) =
              rbt_in_traverse_pairs l1 @ (k1, v1) # rbt_in_traverse_pairs (combine r1 l2) @ (k2, v2) # rbt_in_traverse_pairs r2"
@@ -403,8 +407,6 @@ lemma combine_in_traverse_pairs [rewrite]:
     @end @end @end
   @endgoal @end
 @qed
-
-setup {* fold del_prfstep_thm @{thms combine.simps} *}
 
 section {* Deletion *}
 
@@ -420,32 +422,41 @@ fun del :: "'a::linorder \<Rightarrow> ('a, 'b) rbt \<Rightarrow> ('a, 'b) rbt" 
        if r = Leaf then Node l R k v Leaf
        else if cl r = B then balR l k v (del x r)
        else Node l R k v (del x r))"
-setup {* fold add_rewrite_rule @{thms del.simps} *}
+setup {* add_rewrite_rule @{thm del.simps(1)} *}
+setup {* add_unfolding_rule @{thm del.simps(2)} *}
 
 lemma del_bd:
   "bd_inv t \<Longrightarrow> cl_inv t \<Longrightarrow> bd_inv (del x t) \<and> (
     if cl t = R then black_depth (del x t) = black_depth t
     else black_depth (del x t) = black_depth t - 1)"
-@proof @induct t @with @subgoal "t = Node l c k v r"
-  @case "x = k" @case "x < k" @with
-    @case "l = Leaf" @case "cl l = B" @end
-  @case "x > k" @with
-    @case "r = Leaf" @case "cl r = B" @end
+@proof @induct t @with
+  @subgoal "t = Node l c k v r"
+    @unfold "del x (Node l c k v r)"
+    @case "x = k" @case "x < k" @with
+      @case "l = Leaf" @case "cl l = B" @end
+    @case "x > k" @with
+      @case "r = Leaf" @case "cl r = B" @end
   @endgoal @end
 @qed
 setup {* add_forward_prfstep_cond @{thm del_bd} [with_term "del ?x ?t"] *}
 
 lemma del_cl:
   "cl_inv t \<Longrightarrow> if cl t = R then cl_inv (del x t) else cl_inv' (del x t)"
-@proof @induct t @with @subgoal "t = Node l c k v r"
-  @case "x = k" @case "x < k"
+@proof @induct t @with
+  @subgoal "t = Node l c k v r"
+    @unfold "del x (Node l c k v r)"
+    @case "x = k" @case "x < k"
   @endgoal @end
 @qed
 setup {* add_forward_prfstep_cond @{thm del_cl} [with_term "del ?x ?t"] *}
 
 lemma del_in_traverse_pairs [rewrite]:
   "rbt_sorted t \<Longrightarrow> rbt_in_traverse_pairs (del x t) = remove_elt_pairs x (rbt_in_traverse_pairs t)"
-@proof @induct t @qed
+@proof @induct t @with
+  @subgoal "t = Node l c k v r"
+    @unfold "del x (Node l c k v r)"
+  @endgoal @end
+@qed
 
 definition delete :: "'a::linorder \<Rightarrow> ('a, 'b) rbt \<Rightarrow> ('a, 'b) rbt" where [rewrite]:
   "delete x t = paint B (del x t)"
@@ -459,9 +470,9 @@ theorem delete_sorted [forward]:
 theorem delete_rbt_map [rewrite]:
   "rbt_sorted t \<Longrightarrow> rbt_map (delete x t) = delete_map x (rbt_map t)" by auto2
 
-setup {* del_prfstep "RBT.balance_case" *}
-setup {* del_prfstep "RBT.balL_case" *}
-setup {* del_prfstep "RBT.balR_case" *}
-setup {* del_prfstep "RBT.paint_case" *}
+setup {* del_prfstep "RBTree.balance_case" *}
+setup {* del_prfstep "RBTree.balL_case" *}
+setup {* del_prfstep "RBTree.balR_case" *}
+setup {* del_prfstep "RBTree.paint_case" *}
 
 end
